Added invariant on timestamp of 1b packet, and made phase1 invariant inductive

ironfleet/src/Dafny/Distributed/Protocol/RSL/PerformanceProof/PerformanceProof.i.dfy
@@ -15,7 +15,8 @@ import opened CommonProof__Constants_i
 
 predicate RslAssumption(s:TimestampedRslState)
 {
-  |s.t_replicas| > 0
+  && NoPacketDuplication(s)
+  && |s.t_replicas| > 0
 
   // TODO: Remove this assumption
   && (var nextStep := s.t_environment.nextStep; nextStep.LEnvStepHostIos? ==>
@@ -79,9 +80,16 @@ predicate InitInvariant(s:TimestampedRslState)
   && s.t_replicas[idx].v.replica.learner.unexecuted_learner_state == map[]
   )
 
-  && (forall pkt :: pkt in s.t_environment.sentPackets
+  && (forall pkt :: pkt in s.undeliveredPackets
   ==> pkt.msg.v.RslMessage_Heartbeat?
   )
+}
+
+predicate No1aToDst(undeliveredPackets:multiset<TimestampedLPacket<EndPoint, RslMessage>>, dst:NodeIdentity)
+{
+  && (forall pkt :: pkt in undeliveredPackets
+    && pkt.msg.v.RslMessage_1a?
+    ==> pkt.dst != dst)
 }
 
 predicate Phase1Invariant(s:TimestampedRslState)
@@ -105,36 +113,41 @@ predicate Phase1Invariant(s:TimestampedRslState)
     && s.t_replicas[0].v.replica.proposer.current_state == 1
   )
 
-  && (forall pkt :: pkt in s.t_environment.sentPackets
+  && (forall pkt :: pkt in s.undeliveredPackets
   ==>
    || pkt.msg.v.RslMessage_Heartbeat?
    || pkt.msg.v.RslMessage_1a?
    || pkt.msg.v.RslMessage_1b?
   )
 
-  && (forall pkt :: pkt in s.t_environment.sentPackets
+  && (forall pkt :: pkt in s.undeliveredPackets
   && pkt.msg.v.RslMessage_1b?
   ==> pkt.dst == s.constants.config.replica_ids[0]
+  // && TimeLe(pkt.msg.ts, TimeBound1bSent())
   )
 
-  && (forall pkt :: pkt in s.t_environment.sentPackets
+  && (forall pkt :: pkt in s.undeliveredPackets
       && pkt.msg.v.RslMessage_1a?
    ==> TimeLe(pkt.msg.ts, TimeBound1aSent())
-      && (|s.t_replicas| > 0 ==> pkt.msg.v.bal_1a == s.t_replicas[0].v.replica.proposer.max_ballot_i_sent_1a)
       && pkt.msg.v.bal_1a == Ballot(1, 0)
       && pkt.src == s.constants.config.replica_ids[0]
+
+      && (var undeliveredPackets' := s.undeliveredPackets - multiset({pkt});
+          No1aToDst(undeliveredPackets', pkt.dst)
+        )
   )
 
   && (forall idx :: 0 < idx < |s.t_replicas|
   ==>
-  (s.t_replicas[idx].v.replica.acceptor.max_bal == Ballot(0, 0)
-  ==>
-  LSchedulerTimeBound(s.t_replicas[idx])
-  )
-  //else
-    //(&& s.t_replicas[idx].v.replica.acceptor.max_bal == s.t_replicas[0].v.replica.proposer.max_ballot_i_sent_1a
-    //&& true // TimeLe(s.t_replicas[idx].ts, TimeBound1aReceived())
-    //)
+  if s.t_replicas[idx].v.replica.acceptor.max_bal == Ballot(0, 0) then
+    LSchedulerTimeBound(s.t_replicas[idx])
+  else
+    (forall pkt :: pkt in s.undeliveredPackets
+    && pkt.msg.v.RslMessage_1a?
+    ==> pkt.dst != s.constants.config.replica_ids[idx]
+    // (&& s.t_replicas[idx].v.replica.acceptor.max_bal == s.t_replicas[0].v.replica.proposer.max_ballot_i_sent_1a
+    // && true // TimeLe(s.t_replicas[idx].ts, TimeBound1aReceived())
+    )
   )
 }
 
@@ -143,6 +156,12 @@ lemma lemma_RslInitImpliesInitInv(s:TimestampedRslState)
   requires TimestampedRslInit(s.constants, s);
   ensures InitInvariant(s);
 {
+}
+
+function MultisetToSet<S(!new)>(m:multiset<S>) : set<S>
+  ensures forall x :: x in m <==> x in MultisetToSet(m)
+{
+  set x | x in m :: x
 }
 
 lemma lemma_0_1_InitGoesToPhase1(s:TimestampedRslState, s':TimestampedRslState, j:int)
@@ -161,14 +180,16 @@ lemma lemma_0_1_InitGoesToPhase1(s:TimestampedRslState, s':TimestampedRslState, 
   requires InitInvariant(s)
   ensures Phase1Invariant(s')
 {
-  forall pkt | pkt in s'.t_environment.sentPackets
-      && pkt.msg.v.RslMessage_1a?
-  {
-    assert TimeLe(pkt.msg.ts, TimeBound1aSent());
-    assert pkt.msg.v.bal_1a == s'.t_replicas[0].v.replica.proposer.max_ballot_i_sent_1a;
-    assert BalLt(Ballot(0, 0), pkt.msg.v.bal_1a);
-    assert pkt.src == s.constants.config.replica_ids[0];
-  }
+  // var ios := s.t_environment.nextStep.ios;
+  // var newPacketsSeq := ExtractSentPacketsFromIos(ios);
+  // var newPackets := set x | (x in s'.undeliveredPackets && x !in s.undeliveredPackets) :: x;
+
+  // assume (MultisetToSet(s'.undeliveredPackets) - MultisetToSet(s.undeliveredPackets)) <= (set io | io in ios && io.LIoOpSend? :: io.s);
+  // assume newPackets <= (set io | io in ios && io.LIoOpSend? :: io.s);
+  // assume forall pkt :: (pkt in s'.undeliveredPackets && pkt !in s.undeliveredPackets) ==> ;
+  // assert forall pkt :: pkt in newPackets ==> pkt.msg.v.RslMessage_1a?;
+  // D := (A - B) + C
+  // (D - A) <= C
 
 }
 
@@ -198,6 +219,35 @@ lemma lemma_InitGoesToInitOrPhase1(s:TimestampedRslState, s':TimestampedRslState
   }
 }
 
+lemma lemma_0_j_Phase1GoesToPhase1(s:TimestampedRslState, s':TimestampedRslState, j:int)
+  requires RslAssumption(s);
+  requires ViewAlwaysZero(s)
+  requires RslConsistency(s);
+  requires RslConsistency(s');
+  requires 0 <= j < |s.constants.config.replica_ids|
+
+  requires j > 0;
+
+  requires s.t_environment.nextStep.LEnvStepHostIos?;
+  requires s.t_environment.nextStep.actor == s.constants.config.replica_ids[j];
+  requires s.t_environment.nextStep.nodeStep == RslStep(0)
+
+  requires TimestampedRslNextOneReplica(s, s', j, s.t_environment.nextStep.ios);
+
+  requires Phase1Invariant(s)
+  ensures Phase1Invariant(s')
+{
+  assert ReplicasDistinct(s.constants.config.replica_ids, 0, j);
+  var ios := s.t_environment.nextStep.ios;
+  if ios[0].LIoOpReceive? {
+    // assert s.t_replicas[j].v.replica.acceptor.max_bal == Ballot(0, 0);
+    assert ios[0].r.msg.v.RslMessage_1a?;
+    BoundedLagImpliesBoundedProcessingTime(s.t_replicas[j].dts, s.t_replicas[j].ts, ios[0].r.msg.ts, s'.t_replicas[j].ts);
+  } else {
+    assert Phase1Invariant(s');
+  }
+}
+
 lemma lemma_a_j_Phase1GoesToPhase1(s:TimestampedRslState, s':TimestampedRslState, j:int)
   requires RslAssumption(s);
   requires ViewAlwaysZero(s)
@@ -209,6 +259,7 @@ lemma lemma_a_j_Phase1GoesToPhase1(s:TimestampedRslState, s':TimestampedRslState
 
   requires s.t_environment.nextStep.LEnvStepHostIos?;
   requires s.t_environment.nextStep.actor == s.constants.config.replica_ids[j];
+  requires s.t_environment.nextStep.nodeStep != RslStep(0)
 
   requires TimestampedRslNextOneReplica(s, s', j, s.t_environment.nextStep.ios);
 
